src/Notations.v
@@ -13,6 +13,7 @@
 (** printing =] $\ensuremath{\sqsupseteq}$ *)
 
 Reserved Notation "x * y" (at level 40, left associativity).
+Reserved Notation "x ** y" (at level 40, left associativity).
 Reserved Notation "x 'o' y" (at level 30, right associativity).
 Reserved Notation "x || y" (at level 50, left associativity).
 Reserved Notation "x (+) y" (at level 45, no associativity).
